skip_list/spec/insert.v
@@ -1,0 +1,300 @@
+From iris.algebra Require Import auth frac_auth gset.
+From iris.heap_lang Require Import proofmode.
+
+From SkipList.lib Require Import lock misc.
+From SkipList.skip_list Require Import node_rep code key_equiv.
+From SkipList.skip_list.inv Require Import lazy_inv skip_inv.
+From SkipList.skip_list.spec Require Import find.
+
+
+Local Open Scope Z.
+Module AddSpec (Params: SKIP_LIST_PARAMS).
+  Import Params.
+  Module Find := FindSpec Params.
+  Import Find.
+
+  Section Proofs.
+    Context `{!heapGS Σ, !gset_list_unionGS Σ, !lockG Σ} (lvlN : namespace).
+
+    Theorem findLock_spec (head curr: node_rep) (key: Z)
+      (Γ: lazy_gname) (P: node_rep → iProp Σ) :
+      {{{ 
+        inv lvlN (lazy_list_inv head Γ P)
+        ∗
+        (⌜ curr = head ⌝ ∨ own (s_auth Γ) (◯ {[curr]}))
+        ∗
+        ⌜ node_key curr < key < INT_MAX ⌝
+      }}}
+        findLock (rep_to_node curr) #key
+      {{{ pred succ, RET SOMEV ((rep_to_node pred), (rep_to_node succ));
+        ⌜ node_key pred < key ≤ node_key succ ⌝
+        ∗
+        (⌜ pred = head ⌝ ∨ own (s_auth Γ) (◯ {[pred]}))
+        ∗
+        (own (s_auth Γ) (◯ {[succ]}) ∨ ⌜ succ = tail ⌝)
+        ∗
+        ∃ (l: loc) (γ: gname), ⌜ node_next pred = Some l ⌝
+                               ∗
+                               is_lock γ (node_lock pred) (node_inv l (s_tok Γ) (node_key pred))
+                               ∗
+                               l ↦{#1 / 2} (rep_to_node succ)
+                               ∗
+                               own (s_tok Γ) (GSet (Zlt_range (node_key pred) (node_key succ)))
+                               ∗
+                               locked γ
+      }}}.
+    Proof.
+      iIntros (Φ) "(#Hinv & Hown_curr & Hrange) HΦ".
+      iRevert (curr) "Hown_curr Hrange".
+      iLöb as "IH". 
+      iIntros (curr) "#Hown_curr %Hrange".
+      
+      wp_lam. wp_let.
+      wp_apply (find_frac_spec with "[Hown_curr]").
+      { by iFrame "#". }
+      iIntros (pred succ) "(%Hrange' & #Hown_pred & #Hown_succ & Hlock)".
+      iDestruct "Hlock" as (l γ) "(%Hsome & #Hlock)".
+      wp_pures. wp_lam. wp_pures.
+
+      wp_bind (acquire _).
+      iApply (acquire_spec with "Hlock"); first done.
+      iNext; iIntros (v) "(Hnode & Hlocked)".
+      wp_pures. wp_lam. wp_pures.
+      rewrite Hsome; wp_match.
+      iDestruct "Hnode" as (rep) "(Hnode & Hown_tok_range)".
+
+      wp_bind (Load _).
+      iInv lvlN as (S Skeys L) "(>%Hperm & >%Hsort & >%Hequiv & Hown_auth & Hown_frac & Hown_tok & Hlist)" "Hclose".
+
+      iMod "Hown_auth"; iAssert ((⌜ pred = head ∨ pred ∈ S ⌝ ∗ ⌜succ ∈ S ∨ succ = tail⌝)%I) 
+        with "[Hown_auth Hown_pred Hown_succ]" as "(%Hpred_range & %Hsucc_range)".
+      {
+        iSplit.
+        - iDestruct "Hown_pred" as "[Heq|Hown]"; first by iLeft.
+          iDestruct (own_valid_2 with "Hown_auth Hown") 
+            as %[Hvalid%gset_included]%auth_both_valid_discrete.
+          iPureIntro; right; set_solver.
+        - iDestruct "Hown_succ" as "[Hown|Heq]"; last by iRight.
+          iDestruct (own_valid_2 with "Hown_auth Hown") 
+            as %[Hvalid%gset_included]%auth_both_valid_discrete.
+          iPureIntro; left; set_solver.
+      }
+
+      rewrite (list_equiv_invert L head pred); last first.
+      { by rewrite -elem_of_list_In Hperm elem_of_elements. }
+      iDestruct "Hlist" as (succ' l' γ') "(>%Hsucc'_in_L & >%Hsome' & Hpt & _ & Himp)".
+      assert (l = l') as <- by congruence.
+
+      wp_load.
+      iDestruct (mapsto_agree with "Hnode Hpt") as "%Hsucc".
+      assert (rep = succ') as -> by by apply rep_to_node_inj.
+      iMod ("Hclose" with "[Hpt Himp Hown_auth Hown_frac Hown_tok]").
+      {
+        iNext. iExists S, Skeys, L.
+        iPoseProof ("Himp" with "Hpt") as "Hlist".
+        by iFrame.
+      }
+
+      iModIntro. wp_let. wp_lam. wp_pures. wp_lam. wp_pures.
+      case_bool_decide as Heq; wp_if.
+      + wp_pures. iApply "HΦ". iModIntro; iFrame "# ∗".
+        iSplit. done. iExists l, γ.
+        assert (succ = succ') as <-; last by iFrame "# ∗".
+        apply (sorted_node_key_unique (L ++ [tail])).
+        - apply node_rep_sorted_app in Hsort; by destruct Hsort.
+        - by rewrite in_inv_rev -elem_of_list_In Hperm elem_of_elements.
+        - by apply in_inv_rev. 
+        - congruence.
+      + wp_lam. wp_pures.
+        wp_apply (release_spec with "[Hnode Hlocked Hown_tok_range]"); first done.
+        { iFrame "# ∗"; iExists succ'; iFrame. }
+        iIntros. wp_pures.
+        by iApply ("IH" with "HΦ").
+    Qed.
+
+    Theorem tryInsert_spec (curr head: node_rep) (key: Z) 
+      (q: frac) (Skeys: gset Z) (Γ: lazy_gname) :
+      {{{
+        is_lazy_list lvlN head q Skeys Γ from_bot_list
+        ∗
+        (⌜ curr = head ⌝ ∨ own (s_auth Γ) (◯ {[curr]}))
+        ∗
+        ⌜ node_key curr < key < INT_MAX ⌝
+      }}}
+        tryInsert (rep_to_node curr) #key
+      {{{ v new, RET v;
+        is_lazy_list lvlN head q (Skeys ∪ {[key]}) Γ from_bot_list
+        ∗
+        ( 
+          ⌜ v = NONEV ⌝ ∨ 
+          ( 
+            ⌜ v = SOMEV (rep_to_node new) ⌝ 
+            ∗ 
+            ⌜ node_key new = key ⌝
+          )
+        )
+      }}}.
+    Proof.
+      iIntros (Φ) "(Hlazy & #Hown_curr & %Hrange) HΦ".
+      iDestruct "Hlazy" as (Sfrag) "(%Hequiv & Hown_frag & #Hinv)".
+      wp_lam. wp_let.
+
+      wp_apply findLock_spec.
+      { by iFrame "#". }
+      iIntros (pred succ) "(%Hrange' & #Hown_pred & #Hown_succ & Hlock)".
+      iDestruct "Hlock" as (l γ) "(%Hsome & #Hlock & Hpt & Hown_tok_range & Hlocked)".
+
+      wp_pures. wp_lam. wp_pures.
+      case_bool_decide as Hcase; wp_if.
+      + wp_lam. wp_bind (Snd _).
+        iDestruct "Hown_succ" as "[Hown_succ|%Hsucc]"; last first.
+        { 
+          subst; exfalso. inversion Hcase as [Heq]. 
+          rewrite /node_key/tail//= in Heq; lia. 
+        }
+
+        iInv lvlN as (S Skeys' L) "(>%Hperm & >%Hsort & >%Hequiv' & Hown_auth & Hown_frac & Hown_tok & Hlist)" "Hclose".
+        iMod "Hown_auth"; iDestruct (own_valid_2 with "Hown_auth Hown_succ") 
+          as %[Hvalid%gset_included]%auth_both_valid_discrete.
+        iMod "Hown_frac"; iDestruct (own_valid_2 with "Hown_frac Hown_frag") 
+          as %Hsub%frac_auth_included_total%gset_included.
+        iMod (own_update_2 with "Hown_frac Hown_frag") as "[Hown_frac Hown_frag]".
+        { apply frac_auth_update, (gset_local_update_union _ _ {[ succ ]}). }
+        iMod "Hown_tok".
+
+        wp_pures.
+        iMod ("Hclose" with "[Hlist Hown_auth Hown_frac Hown_tok]") as "_".
+        {
+          iNext. iExists S, Skeys', L.
+          assert (S ∪ {[ succ ]} ≡ S) as -> by set_solver.
+          by iFrame.
+        }
+        iModIntro.
+
+        wp_apply (release_spec with "[Hlock Hpt Hown_tok_range Hlocked]"); first done.
+        { iFrame "# ∗"; iExists succ; iFrame. }
+        iIntros "_". wp_pures.
+        iModIntro. iApply "HΦ".
+        iSplit; last by iLeft.
+        iExists (Sfrag ∪ {[succ]}). 
+        iFrame "# ∗". iPureIntro.
+
+        assert (key = node_key succ) as -> by congruence.
+        assert (key_equiv {[ succ ]} {[ node_key succ ]}) as Hequiv''.
+        { rewrite /key_equiv ?elements_singleton //. }
+        assert (Skeys ⊆ Skeys') as HsubSkeys.
+        { by apply (key_equiv_subseteq Sfrag S). }
+        assert ({[ node_key succ ]} ⊆ Skeys') as Hsub_succ.
+        { by apply (key_equiv_subseteq {[ succ ]} S). }
+        assert (Skeys ∪ {[ node_key succ ]} ⊆ Skeys') as Hsub_union_Skeys.
+        { by apply union_subseteq. }
+        assert (Sfrag ∪ {[ succ ]} ⊆ S) as Hsub_union_S.
+        { by apply union_subseteq. }
+        by apply (key_equiv_union S Sfrag {[ succ ]} Skeys' Skeys {[ node_key succ ]}).
+      + wp_lam. wp_pures.
+        rewrite Hsome; wp_match.
+        wp_load. wp_let. wp_alloc l' as "Hpt'". wp_let.
+        iDestruct "Hpt'" as "(Hpt' & Hpt'_dup)".
+
+        assert (key ≠ node_key succ) as Hneq by congruence.
+        rewrite (Zlt_range_split_op (node_key pred) (node_key succ) key); last lia.
+        iDestruct "Hown_tok_range" as "((Htok_range1 & Htok_range2) & Htok_k)".
+
+        wp_apply (newlock_spec (node_inv l' (s_tok Γ) key) with "[Hpt'_dup Htok_range2]").
+        { iExists succ; iFrame. }
+        iIntros (lk) "#Hlock'". iDestruct "Hlock'" as (γ') "Hlock'".
+        wp_pures.
+
+        rewrite (fold_rep_to_node (key, Some l', None, lk)).
+        set (new := (key, Some l', None, lk)).
+        
+        wp_bind (Store _ _).
+        iInv lvlN as (S Skeys' L) "(>%Hperm & >%Hsort & >%Hequiv' & Hown_auth & Hown_frac & Hown_tok & Hlist)" "Hclose".
+        iMod "Hown_auth"; iMod "Hown_frac"; iMod "Hown_tok".
+
+        iAssert ((⌜ pred = head ∨ pred ∈ S ⌝)%I) 
+          with "[Hown_auth Hown_pred]" as %Hpred_range.
+        {
+          iDestruct "Hown_pred" as "[Heq|Hown]"; first by iLeft.
+          iDestruct (own_valid_2 with "Hown_auth Hown") 
+            as %[Hvalid%gset_included]%auth_both_valid_discrete.
+          iPureIntro; right; set_solver.
+        }
+
+        rewrite (list_equiv_insert head pred new succ L l l' γ'); first last.
+        { by rewrite -elem_of_list_In Hperm elem_of_elements. }
+        { auto. }
+        { rewrite /node_key//=; rewrite /node_key in Hrange'; rewrite /node_key in Hneq; lia. }
+        { rewrite /node_key//=; lia. }
+
+        iDestruct ("Hlist" with "[Hpt Hpt' Hlock]") as "Hlist".
+        { iNext. unfold from_bot_list. by iFrame "# ∗". }
+        iDestruct "Hlist" as (L') "(Hpt & Hsort & Hperm & Himp)".
+        iMod "Hsort" as %Hsort'; iMod "Hperm" as %Hperm'; iMod "Hpt".
+        wp_store.
+
+        iDestruct (own_valid_2 with "Hown_frac Hown_frag") 
+          as %HsubS%frac_auth_included_total%gset_included.
+        iDestruct (own_valid_2 with "Hown_tok Htok_k") as 
+            %Hdisj%gset_disj_valid_op.
+        iMod (own_update_2 with "Hown_frac Hown_frag") as "[Hown_frac Hown_frac_frag]".
+        { apply frac_auth_update, (gset_local_update_union _ _ {[ new ]}). }
+        iMod (own_update with "Hown_auth") as "[Hown_auth Hown_auth_frag]".
+        { apply auth_update_alloc, (gset_local_update_union _ _ {[ new ]}). }
+        
+        iCombine "Hown_tok Htok_k" as "Hown_tok". 
+        rewrite gset_disj_union; last done.
+
+        assert (Skeys ⊆ Skeys') as HsubSkeys.
+        { by apply (key_equiv_subseteq Sfrag S). }
+
+        iDestruct "Hpt" as "(Hpt & Hpt_dup)".
+        iMod ("Hclose" with "[Hpt_dup Himp Hown_auth Hown_frac Hown_tok]") as "_".
+        {
+          iNext. iExists _, _, L'. 
+          iPoseProof ("Himp" with "Hpt_dup") as "Hlist".
+          iFrame. iPureIntro. split; last first.
+          {
+            split; first done.
+            apply key_equiv_insert_nin; auto.
+            set_solver.
+          }
+
+          apply NoDup_Permutation.
+          { 
+            apply node_rep_sorted_app in Hsort'; destruct Hsort' as [_ Hsort']. 
+            apply node_rep_sorted_app in Hsort'; destruct Hsort' as [Hsort' _].
+            by apply sorted_node_lt_no_dup.
+          } 
+          { apply NoDup_elements. }
+
+          simpl in Hperm'; apply Permutation_cons_inv in Hperm'.
+          intros x; split.
+          - rewrite elem_of_elements Hperm' elem_of_list_In.
+            intros Hin. destruct Hin as [Heq|Hin].
+            * set_solver.
+            * apply elem_of_union_l. 
+              by rewrite -elem_of_elements -Hperm elem_of_list_In.
+          - rewrite elem_of_elements Hperm'. 
+            intros Hin. apply elem_of_union in Hin as [Hin|Heq].
+            * rewrite elem_of_list_In. right.
+              by rewrite -elem_of_list_In Hperm elem_of_elements.
+            * set_solver.
+        }
+
+        iModIntro. wp_pures. wp_lam. wp_pures.
+        wp_apply (release_spec with "[Hlock Hpt Hlocked Htok_range1]"); first done.
+        { iFrame "# ∗"; iExists new; iFrame. }
+        iIntros "_". wp_pures. 
+        iModIntro. iApply "HΦ".
+        iSplit; last by iRight.
+        iExists (Sfrag ∪ {[new]}).
+        iFrame "# ∗". iPureIntro.
+        apply key_equiv_insert_nin; auto.
+        set_solver.
+
+        Unshelve. auto. (* Why ;-; *)
+    Qed.
+
+  End Proofs.
+End AddSpec.
